theories/demo/demo2.v
@@ -53,21 +53,21 @@ Definition defs := [{
   obliv olist (:nat) :=
     case unfold<nat> $0 of
       𝟙
-    | 𝟙 ~+ ~𝔹 * (olist@$0);
+    | 𝟙 ~+ ~𝔹 * (olist $0);
 
-  def s_list :{⊥} Π~:list, Π:nat, olist@$0 :=
+  def s_list :{⊥} Π~:list, Π:nat, olist $0 :=
     \~:list => \:nat =>
       case unfold<nat> $0 of
         ()
       | tape (case unfold<list> $2 of
-                ~inl<𝟙 ~+ ~𝔹 * (olist@$1)> ()
-              | ~inr<𝟙 ~+ ~𝔹 * (olist@$1)> (tape (s𝔹 ($0).1, s_list ($0).2 $1)));
+                ~inl<𝟙 ~+ ~𝔹 * (olist $1)> ()
+              | ~inr<𝟙 ~+ ~𝔹 * (olist $1)> (tape (s𝔹 ($0).1, s_list ($0).2 $1)));
 
-  def r_list :{⊤} Π:nat, Π:olist@$0, list :=
+  def r_list :{⊤} Π:nat, Π:olist $0, list :=
     \:nat =>
       case unfold<nat> $0 of
         \:𝟙 => nil
-      | \:𝟙 ~+ ~𝔹 * (olist@$0) =>
+      | \:𝟙 ~+ ~𝔹 * (olist $0) =>
           ~case $0 of
             nil
           | cons (r𝔹 ($0).1, r_list $2 ($0).2)
