theories/demo/demo3.v
@@ -83,21 +83,21 @@ Definition defs := [{
   obliv ~list (:nat) :=
     case unfold<nat> $0 of
       𝟙
-    | 𝟙 ~+ ~V * (~list@$0);
+    | 𝟙 ~+ ~V * (~list $0);
 
-  def s_list :{⊥} Π~:list, Π:nat, ~list@$0 :=
+  def s_list :{⊥} Π~:list, Π:nat, ~list $0 :=
     \~:list => \:nat =>
       case unfold<nat> $0 of
         ()
       | tape (case unfold<list> $2 of
-                ~inl<𝟙 ~+ ~V * (~list@$1)> ()
-              | ~inr<𝟙 ~+ ~V * (~list@$1)> (tape (s_V ($0).1, s_list ($0).2 $1)));
+                ~inl<𝟙 ~+ ~V * (~list $1)> ()
+              | ~inr<𝟙 ~+ ~V * (~list $1)> (tape (s_V ($0).1, s_list ($0).2 $1)));
 
-  def r_list :{⊤} Π:nat, Π:~list@$0, list :=
+  def r_list :{⊤} Π:nat, Π:~list $0, list :=
     \:nat =>
       case unfold<nat> $0 of
         \:𝟙 => nil
-      | \:𝟙 ~+ ~V * (~list@$0) =>
+      | \:𝟙 ~+ ~V * (~list $0) =>
           ~case $0 of
             nil
           | cons (r_V ($0).1, r_list $2 ($0).2);
@@ -105,11 +105,11 @@ Definition defs := [{
   (* The public view is the upper bound of the number of its vertices. The
   oblivious representation is essentially the flatten tree. So [~tree] is simply
   an alias of [~list]. *)
-  def s_tree :{⊥} Π~:tree, Π:nat, ~tree@$0 :=
+  def s_tree :{⊥} Π~:tree, Π:nat, ~tree $0 :=
     \~:tree => \:nat => s_list (tolist $1) $0;
 
-  def r_tree :{⊤} Π:nat, Π:~tree@$0, tree :=
-    \:nat => \:~tree@$0 => fromlist (r_list $1 $0);
+  def r_tree :{⊤} Π:nat, Π:~tree $0, tree :=
+    \:nat => \:~tree $0 => fromlist (r_list $1 $0);
 
   def tolist :{⊤} Π~:tree, list :=
     \~:tree =>
